WIP: PF to V

src/equiv/TsoPFtoV.v
@@ -21,7 +21,6 @@ Require Import PromisingArch.promising.TsoPromising.
 
 Set Implicit Arguments.
 
-
 (* TODO: move *)
 Require Import ClassicalChoice.
 
@@ -36,14 +35,398 @@ Inductive opt_rel3 A B C (rel: A -> B -> C -> Prop): forall (a:option A) (b:opti
 .
 Hint Constructors opt_rel3.
 
-(* TODO: move *)
-Definition adj A (rel: A -> A -> Prop) (l: list A): Prop :=
-  forall i prev next
-    (PREV: nth_error l i = Some prev)
-    (NEXT: nth_error l (S i) = Some next),
-    rel prev next.
+Inductive sim_memory (n: nat) (mem_pf mem_v: Memory.t): Prop :=
+| sim_memory_intro
+    mem_post
+    (MEMORY: mem_pf = mem_v ++ mem_post)
+    (LENGTH: List.length mem_v = n)
+.
+Hint Constructors sim_memory.
 
-(* TODO: Machine equality seems to be possible like VtoP *)
+Inductive sim_local (n: nat) (lc_pf lc_v: Local.t): Prop :=
+| sim_local_intro
+    (COH: lc_pf.(Local.coh) = lc_v.(Local.coh))
+    (VRN: lc_pf.(Local.vrn) = lc_v.(Local.vrn))
+    (LPER: lc_pf.(Local.lper) = lc_v.(Local.lper))
+    (PER: lc_pf.(Local.per) = lc_v.(Local.per))
+    (PROMISES_PF: forall ts (PROMISE: Promises.lookup ts lc_pf.(Local.promises) = true), ts > n)
+    (PROMISES_V: lc_v.(Local.promises) = fun _ => false)
+.
+Hint Constructors sim_local.
+
+Inductive sim_sl (n: nat) (sl_pf sl_v: State.t (A:=unit) * Local.t): Prop :=
+| sim_sl_intro
+    (STATE: fst sl_pf = fst sl_v)
+    (LOCAL: sim_local n (snd sl_pf) (snd sl_v))
+.
+Hint Constructors sim_sl.
+
+Inductive sim (n: nat) (m_pf m_v: Machine.t): Prop :=
+| sim_intro
+    (TPOOL: forall tid, opt_rel (sim_sl n)
+                           (IdMap.find tid m_pf.(Machine.tpool))
+                           (IdMap.find tid m_v.(Machine.tpool)))
+    (MEMORY: sim_memory n m_pf.(Machine.mem) m_v.(Machine.mem))
+.
+Hint Constructors sim.
+
+Definition promises_le (tid: Id.t) (promises: Promises.t) (mem: Memory.t): Prop :=
+  forall ts (LOOKUP: Promises.lookup ts promises = true),
+  exists loc val, Memory.get_msg ts mem = Some (Msg.mk loc val tid).
+
+Inductive promises_wf (n: nat) (m: Machine.t): Prop :=
+| promises_wf_intro
+    (SOUND: forall tid st lc
+              (FIND: IdMap.find tid m.(Machine.tpool) = Some (st, lc)),
+        <<LE: promises_le tid lc.(Local.promises) m.(Machine.mem)>>)
+    (COMPLETE: forall ts loc val tid
+           (GT: n < ts)
+           (GET: Memory.get_msg ts m.(Machine.mem) = Some (Msg.mk loc val tid)),
+        exists st lc,
+          (<<FIND: IdMap.find tid m.(Machine.tpool) = Some (st, lc)>>) /\
+          (<<IN: Promises.lookup ts lc.(Local.promises) = true>>))
+.
+Hint Constructors promises_wf.
+
+
+
+Lemma sim_memory_latest
+      n mem_pf mem_v loc from to
+      (SIM: sim_memory n mem_pf mem_v)
+      (TO: to <= n)
+      (LATEST: Memory.latest loc from to mem_pf):
+  Memory.latest loc from to mem_v.
+Proof.
+  inv SIM. ii. exploit LATEST; eauto.
+  rewrite nth_error_app1; ss. nia.
+Qed.
+
+Lemma sim_memory_read
+      n mem_pf mem_v loc ts val
+      (SIM: sim_memory n mem_pf mem_v)
+      (TS: ts <= n)
+      (READ: Memory.read loc ts mem_pf = val):
+  Memory.read loc ts mem_v = val.
+Proof.
+  inv SIM. unfold Memory.read in *.
+  destruct ts; ss.
+  des_ifs; rewrite nth_error_app1 in *; try nia; congr.
+Qed.
+
+Lemma sim_memory_exclusive
+      n mem_pf mem_v tid loc val from
+      (SIM: sim_memory n mem_pf mem_v)
+      (LENGTH: length mem_pf > n)
+      (FROM: from < n + 1)
+      (EXCLUSIVE: Memory.exclusive tid loc from (n + 1) mem_pf):
+  Memory.exclusive tid loc from (n + 1) (mem_v ++ [Msg.mk loc val tid]).
+Proof.
+  inv SIM. ii. des.
+  exploit EXCLUSIVE; eauto.
+  destruct (classic (ts = length mem_v)).
+  { subst. rewrite nth_error_app2 in MSG; try nia.
+    rewrite Nat.sub_diag in MSG. ss. inv MSG. rewrite <- H1 in *. ss. }
+  rewrite nth_error_app1 in *; try nia. ss.
+Qed.
+
+Lemma next_fulfill_exists
+      n m1 m
+      (EXEC1: Machine.state_exec m1 m)
+      (PROMISES1: promises_wf n m1):
+  exists tid st1 lc1 st2 lc2,
+    (<<FIND: IdMap.find tid m1.(Machine.tpool) = Some (st1, lc1)>>) /\
+    (<<STEPS: rtc (ExecUnit.state_step tid)
+                  (ExecUnit.mk st1 lc1 m1.(Machine.mem))
+                  (ExecUnit.mk st2 lc2 m1.(Machine.mem))>>) /\
+    (exists st3 lc3 ord vloc vval res m2,
+        (<<STEP_ST: State.step (Event.write false ord vloc vval res) st2 st3>>) /\
+        (<<STEP_LC: Local.fulfill vloc vval res (n + 1) tid lc2 m1.(Machine.mem) lc3>>) /\
+        (<<MACHINE2: m2 = Machine.mk (IdMap.add tid (st3, lc3) m1.(Machine.tpool)) m1.(Machine.mem)>>) /\
+        (<<EXEC2: Machine.state_exec m2 m>>) /\
+        (<<PROMISES2: promises_wf (n + 1) m2>>)) \/
+    (exists st3 lc3 ordr ordw vloc vold vnew old_ts m2,
+        (<<STEP_ST: State.step (Event.rmw ordr ordw vloc vold vnew) st2 st3>>) /\
+        (<<STEP_LC: Local.rmw vloc vold vnew old_ts (n + 1) tid lc2 m1.(Machine.mem) lc3>>) /\
+        (<<MACHINE2: m2 = Machine.mk (IdMap.add tid (st3, lc3) m1.(Machine.tpool)) m1.(Machine.mem)>>) /\
+        (<<EXEC2: Machine.state_exec m2 m>>) /\
+        (<<PROMISES2: promises_wf (n + 1) m2>>)).
+Proof.
+Admitted.
+
+Lemma sim_step
+      n
+      e tid lc1_pf lc2_pf mem_pf
+      lc1_v mem_v
+      (LOCAL1: sim_local n lc1_pf lc1_v)
+      (MEMORY: sim_memory n mem_pf mem_v)
+      (WF1_PF: Local.wf tid mem_pf lc1_pf)
+      (WF1_V: Local.wf tid mem_v lc1_v)
+      (STEP_PF: Local.step e tid mem_pf lc1_pf lc2_pf):
+  (exists lc2_v,
+      (<<STEP_V: Local.view_step e tid mem_v mem_v lc1_v lc2_v>>) /\
+      (<<LOCAL2: sim_local n lc2_pf lc2_v>>) /\
+      (<<PROMISES_PF: lc2_pf.(Local.promises) = lc1_pf.(Local.promises)>>)) \/
+  (exists loc,
+      <<COH: (lc2_pf.(Local.coh) loc).(View.ts) > n>>).
+Proof.
+  destruct lc1_pf as [coh_pf vrn_pf lper_pf per_pf promises_pf].
+  destruct lc1_v as [coh_v vrn_v lper_v per_v promises_v].
+  dup LOCAL1. inv LOCAL0. ss. subst.
+  inv STEP_PF.
+  - (* internal *)
+    left. esplits; eauto. econs 1; ss.
+  - (* read *)
+    destruct (classic (ts <= n)).
+    + inv STEP. ss. left. esplits.
+      * econs 2; eauto. econs; s; eauto.
+        { eapply sim_memory_latest; eauto.
+          inv WF1_V. inv MEMORY; ss. }
+        { eapply sim_memory_read; eauto. }
+      * eauto.
+      * ss.
+    + inv STEP. ss. right. exists vloc.(ValA.val).
+      rewrite fun_add_spec_eq. ss.
+      unfold Local.read_view. condtac; s.
+      { rewrite <- e in *.
+        eapply le_gt_trans; [eapply join_l|]. nia. }
+      eapply le_gt_trans; [eapply join_r|]. nia.
+  - (* fulfill - promises_wf required *)
+    inv STEP. ss. exploit PROMISES_PF; eauto. i.
+    right. exists vloc.(ValA.val).
+    rewrite fun_add_spec_eq. ss.
+  - (* rmw - promises_wf required *)
+    inv STEP. ss. exploit PROMISES_PF; eauto. i.
+    right. exists vloc.(ValA.val).
+    rewrite fun_add_spec_eq. ss.
+  - (* rmw failure *)
+    destruct (classic (old_ts <= n)).
+    + inv STEP. ss. left. esplits.
+      * econs 5; eauto. econs; s; eauto.
+        { eapply sim_memory_latest; eauto.
+          inv WF1_V. inv MEMORY. ss. }
+        { eapply sim_memory_read; eauto. }
+      * eauto.
+      * ss.
+    + inv STEP. ss. right. exists vloc.(ValA.val).
+      rewrite fun_add_spec_eq. ss.
+      unfold Local.read_view. condtac; s.
+      { rewrite <- e in *.
+        eapply le_gt_trans; [eapply join_l|]. nia. }
+      eapply le_gt_trans; [eapply join_r|]. nia.
+  - (* dmb *)
+    left. inv STEP. inv COHMAX. ss. esplits.
+    + econs 6; eauto. econs; eauto. econs. ss.
+    + eauto.
+    + ss.
+  - (* flush *)
+    left. inv STEP. ss. esplits.
+    + econs 7; eauto. econs; eauto.
+    + eauto.
+    + ss.
+  - (* flushopt *)
+    left. inv STEP. ss. esplits.
+    + econs 8; eauto. econs; eauto.
+    + eauto.
+    + ss.
+Qed.
+
+Lemma sim_fulfill
+      n tid
+      vloc vval res lc1_pf mem_pf lc2_pf
+      lc1_v mem1_v
+      (LOCAL1: sim_local n lc1_pf lc1_v)
+      (MEMORY1: sim_memory n mem_pf mem1_v)
+      (WF1_PF: Local.wf tid mem_pf lc1_pf)
+      (WF1_V: Local.wf tid mem1_v lc1_v)
+      (STEP_PF: Local.fulfill vloc vval res (n + 1) tid lc1_pf mem_pf lc2_pf):
+  exists lc2_v mem2_v,
+    (<<STEP_V: Local.write vloc vval res (n + 1) tid lc1_v mem1_v lc2_v mem2_v>>) /\
+    (<<LOCAL2: sim_local (n + 1) lc2_pf lc2_v>>) /\
+    (<<MEMORY2: sim_memory (n + 1) mem_pf mem2_v>>) /\
+    (<<PROMISES_PF: lc2_pf.(Local.promises) = Promises.unset (n + 1) lc1_pf.(Local.promises)>>).
+Proof.
+  destruct lc1_pf as [coh_pf vrn_pf lper_pf per_pf promises_pf].
+  destruct lc1_v as [coh_v vrn_v lper_v per_v promises_v].
+  inv LOCAL1. inv MEMORY1. inv STEP_PF. ss. subst.
+  esplits.
+  - econs; eauto.
+    unfold Memory.append. rewrite Nat.add_1_r. refl.
+  - econs; eauto; s. i.
+    revert PROMISE0. rewrite Promises.unset_o. condtac; ss. i.
+    exploit PROMISES_PF; eauto. i.
+    destruct (classic (ts = length mem1_v + 1)); try nia. congr.
+  - revert MSG. unfold Memory.get_msg. rewrite Nat.add_1_r. ss.
+    rewrite nth_error_app2; try nia.
+    rewrite Nat.sub_diag.
+    destruct mem_post; ss. i. inv MSG.
+    econs.
+    + rewrite <- app_assoc. ss.
+    + rewrite app_length. s. rewrite Nat.add_1_r. ss.
+  - ss.
+Qed.
+
+Lemma sim_rmw
+      n tid
+      vloc vold vnew old_ts lc1_pf mem_pf lc2_pf
+      lc1_v mem1_v
+      (LOCAL1: sim_local n lc1_pf lc1_v)
+      (MEMORY1: sim_memory n mem_pf mem1_v)
+      (WF1_PF: Local.wf tid mem_pf lc1_pf)
+      (WF1_V: Local.wf tid mem1_v lc1_v)
+      (STEP_PF: Local.rmw vloc vold vnew old_ts (n + 1) tid lc1_pf mem_pf lc2_pf):
+  exists lc2_v mem2_v,
+    (<<STEP_V: Local.vrmw vloc vold vnew old_ts (n + 1) tid lc1_v mem1_v lc2_v mem2_v>>) /\
+    (<<LOCAL2: sim_local (n + 1) lc2_pf lc2_v>>) /\
+    (<<MEMORY2: sim_memory (n + 1) mem_pf mem2_v>>) /\
+    (<<PROMISES_PF: lc2_pf.(Local.promises) = Promises.unset (n + 1) lc1_pf.(Local.promises)>>).
+Proof.
+  destruct lc1_pf as [coh_pf vrn_pf lper_pf per_pf promises_pf].
+  destruct lc1_v as [coh_v vrn_v lper_v per_v promises_v].
+  inv LOCAL1. dup MEMORY1. inv MEMORY0. inv STEP_PF. ss. subst.
+  esplits.
+  - econs.
+    + ss.
+    + ss.
+    + instantiate (1 := mem1_v ++ [Msg.mk vloc.(ValA.val) vnew.(ValA.val) tid]).
+      eapply sim_memory_exclusive; eauto.
+      rewrite app_length.
+      destruct mem_post; s; try nia.
+      rewrite Nat.add_1_r, app_nil_r in MSG.
+      unfold Memory.get_msg in *. ss.
+      exploit nth_error_some; eauto. i. nia.
+    + eapply sim_memory_read; eauto. nia.
+    + ss.
+    + ss.
+    + ss.
+    + unfold Memory.append. rewrite Nat.add_1_r. refl.
+    + ss.
+  - econs; eauto; s. i.
+    revert PROMISE0. rewrite Promises.unset_o. condtac; ss. i.
+    exploit PROMISES_PF; eauto. i.
+    destruct (classic (ts = length mem1_v + 1)); try nia. congr.
+  - revert MSG. unfold Memory.get_msg. rewrite Nat.add_1_r. ss.
+    rewrite nth_error_app2; try nia.
+    rewrite Nat.sub_diag.
+    destruct mem_post; ss. i. inv MSG.
+    econs.
+    + rewrite <- app_assoc. ss.
+    + rewrite app_length. s. rewrite Nat.add_1_r. ss.
+  - ss.
+Qed.
+
+(* TODO: move *)
+
+Lemma rtc_state_step_incr
+      tid eu1 eu2
+      (STEP: rtc (ExecUnit.state_step tid) eu1 eu2):
+  ExecUnit.le eu1 eu2.
+Proof.
+  induction STEP; try refl.
+  exploit ExecUnit.state_step_incr; eauto. i.
+  etrans; eauto.
+Qed.
+
+Lemma sim_next_fulfill
+      n tid
+      mem_pf mem1_v
+      st1 lc1_pf st2 lc2_pf st3 lc3_pf ord vloc vval res
+      lc1_v
+      (MEMORY1: sim_memory n mem_pf mem1_v)
+      (LOCAL1: sim_local n lc1_pf lc1_v)
+      (WF1_PF: Local.wf tid mem_pf lc1_pf)
+      (WF1_V: Local.wf tid mem1_v lc1_v)
+      (STEPS: rtc (ExecUnit.state_step tid)
+                  (ExecUnit.mk st1 lc1_pf mem_pf)
+                  (ExecUnit.mk st2 lc2_pf mem_pf))
+      (STEP_ST: State.step (Event.write false ord vloc vval res) st2 st3)
+      (STEP_LC: Local.fulfill vloc vval res (n + 1) tid lc2_pf mem_pf lc3_pf):
+  exists lc2_v lc3_v mem3_v,
+    (<<STEPS_V: rtc (ExecUnit.view_step tid)
+                    (ExecUnit.mk st1 lc1_v mem1_v)
+                    (ExecUnit.mk st2 lc2_v mem1_v)>>) /\
+    (<<STEP_V: ExecUnit.view_step tid (ExecUnit.mk st2 lc2_v mem1_v) (ExecUnit.mk st3 lc3_v mem3_v)>>) /\
+    (<<LOCAL3: sim_local (n + 1) lc3_pf lc3_v>>) /\
+    (<<MEMORY3: sim_memory (n + 1) mem_pf mem3_v>>) /\
+    (<<PROMISES2_PF: lc2_pf.(Local.promises) = lc1_pf.(Local.promises)>>) /\
+    (<<PROMISES3_PF: lc3_pf.(Local.promises) = Promises.unset (n + 1) lc1_pf.(Local.promises)>>).
+Proof.
+  revert n mem1_v st3 lc3_pf ord vloc vval res lc1_v MEMORY1 LOCAL1 WF1_PF WF1_V STEP_ST STEP_LC.
+  dependent induction STEPS; i.
+  { exploit sim_fulfill; eauto. i. des.
+    esplits; eauto.
+    econs. econs; eauto. econs 3; eauto. }
+  inv H. inv STEP.
+  exploit sim_step; eauto. i. des.
+  - destruct y. ss. subst.
+    exploit Local.step_wf; try exact LOCAL; eauto. i.
+    exploit Local.view_step_wf; try exact STEP_V; eauto. i.
+    exploit IHSTEPS; eauto. i. des.
+    esplits.
+    + econs 2; eauto. econs. econs; eauto.
+    + eauto.
+    + ss.
+    + ss.
+    + congr.
+    + congr.
+  - exfalso.
+    exploit rtc_state_step_incr; try exact STEPS. i.
+    inv STEP_LC. inv WRITABLE. inv COHMAX. inv x0. inv LC. ss.
+    specialize (COH0 loc). specialize (COHMAX0 loc).
+    rewrite COHMAX0 in COH0.
+    exploit le_lt_trans; [exact COH0|exact EXT|]. i. nia.
+Qed.
+      
+Lemma sim_next_rmw
+      n tid
+      mem_pf mem1_v
+      st1 lc1_pf st2 lc2_pf st3 lc3_pf ordr ordw vloc vold vnew old_ts
+      lc1_v
+      (MEMORY1: sim_memory n mem_pf mem1_v)
+      (LOCAL1: sim_local n lc1_pf lc1_v)
+      (WF1_PF: Local.wf tid mem_pf lc1_pf)
+      (WF1_V: Local.wf tid mem1_v lc1_v)
+      (STEPS: rtc (ExecUnit.state_step tid)
+                  (ExecUnit.mk st1 lc1_pf mem_pf)
+                  (ExecUnit.mk st2 lc2_pf mem_pf))
+      (STEP_ST: State.step (Event.rmw ordr ordw vloc vold vnew) st2 st3)
+      (STEP_LC: Local.rmw vloc vold vnew old_ts (n + 1) tid lc2_pf mem_pf lc3_pf):
+  exists lc2_v lc3_v mem3_v,
+    (<<STEPS_V: rtc (ExecUnit.view_step tid)
+                    (ExecUnit.mk st1 lc1_v mem1_v)
+                    (ExecUnit.mk st2 lc2_v mem1_v)>>) /\
+    (<<STEP_V: ExecUnit.view_step tid (ExecUnit.mk st2 lc2_v mem1_v) (ExecUnit.mk st3 lc3_v mem3_v)>>) /\
+    (<<LOCAL3: sim_local (n + 1) lc3_pf lc3_v>>) /\
+    (<<MEMORY3: sim_memory (n + 1) mem_pf mem3_v>>) /\
+    (<<PROMISES2_PF: lc2_pf.(Local.promises) = lc1_pf.(Local.promises)>>) /\
+    (<<PROMISES3_PF: lc3_pf.(Local.promises) = Promises.unset (n + 1) lc1_pf.(Local.promises)>>).
+Proof.
+  revert n mem1_v st3 lc3_pf ordr ordw vloc vold vnew lc1_v MEMORY1 LOCAL1 WF1_PF WF1_V STEP_ST STEP_LC.
+  dependent induction STEPS; i.
+  { exploit sim_rmw; eauto. i. des.
+    esplits; eauto.
+    econs. econs; eauto. econs 4; eauto. }
+  inv H. inv STEP.
+  exploit sim_step; eauto. i. des.
+  - destruct y. ss. subst.
+    exploit Local.step_wf; try exact LOCAL; eauto. i.
+    exploit Local.view_step_wf; try exact STEP_V; eauto. i.
+    exploit IHSTEPS; eauto. i. des.
+    esplits.
+    + econs 2; eauto. econs. econs; eauto.
+    + eauto.
+    + ss.
+    + ss.
+    + congr.
+    + congr.
+  - exfalso.
+    exploit rtc_state_step_incr; try exact STEPS. i.
+    inv STEP_LC. inv WRITABLE. inv COHMAX. inv x0. inv LC. ss.
+    specialize (COH1 loc). specialize (COHMAX0 loc).
+    rewrite COHMAX0 in COH1.
+    exploit le_lt_trans; [exact COH1|exact EXT|]. i. nia.
+Qed.
+
+
 Theorem promising_pf_to_view
         p pm
         (EXEC: Machine.pf_exec p pm):
@@ -51,65 +434,4 @@ Theorem promising_pf_to_view
     <<STEP: Machine.view_exec p vm>> /\
     <<SIM: Machine.equiv pm vm>>.
 Proof.
-  inv EXEC. rename m1 into mf, pm into mt.
-
-  (* TODO: by STEP2 *)
-  (* https://github.com/kaist-cp/promising-hw/issues/46#issuecomment-672911617 1. *)
-  assert (TRACES: forall tid, exists traces,
-               opt_rel3
-                 (fun eu_begin eu_end eus =>
-                    <<BEGIN_END: exists l, eus = eu_begin :: l ++ [eu_end]>> /\
-                    <<ADJ: adj (fun a b => ExecUnit.state_step
-                                          tid
-                                          (ExecUnit.mk (fst a) (snd a) mf.(Machine.mem))
-                                          (ExecUnit.mk (fst b) (snd b) mt.(Machine.mem)))
-                               eus>>)
-                 (IdMap.find tid mf.(Machine.tpool))
-                 (IdMap.find tid mt.(Machine.tpool))
-                 traces).
-  { admit.
-    (* maybe the following may help: https://github.com/kaist-cp/promising-hw/pull/73/files#diff-aa828713167abebc52916701eb636131R72 *)
-  }
-  apply choice in TRACES. des. rename f into traces.
-
-  Inductive event_order
-            (traces: Id.t -> option (list (State.t (A:=unit) * Local.t)))
-            (l r:Id.t * nat)
-    : Prop :=
-  | event_order_intro
-      (* l: lf -> lt in ltrace *)
-      (* r: rf -> rt in rtrace *)
-      ltrace lf lt
-      rtrace rf rt
-      (LTRACE: traces (fst l) = Some ltrace)
-      (RTRACE: traces (fst r) = Some rtrace)
-      (LF: nth_error ltrace (snd l) = Some lf)
-      (RF: nth_error rtrace (snd l) = Some rf)
-      (LT: nth_error ltrace (S (snd l)) = Some lt)
-      (RT: nth_error rtrace (S (snd l)) = Some rt)
-  (* TODO: describe https://github.com/kaist-cp/promising-hw/issues/46#issuecomment-672911617 2. *)
-  (* consult https://github.com/kaist-cp/promising-hw/pull/73/files#diff-aa828713167abebc52916701eb636131R129 *)
-  .
-
-  (* https://github.com/kaist-cp/promising-hw/issues/46#issuecomment-672911617 3. *)
-  assert (acyclic (event_order traces)).
-  { admit. }
-
-  (* the list of all events *)
-  assert (EVENTS: exists events,
-             <<SOUND: forall tid n trace t
-                        (TRACE: traces tid = Some trace)
-                        (TO: nth_error trace (S n) = Some t),
-               In (tid, n) events>> /\
-             <<COMPLETE: forall tid n (IN: In (tid, n) events),
-                 exists trace t,
-                   <<TRACE: traces tid = Some trace>> /\
-                   <<TO: nth_error trace (S n) = Some t>>>>).
-  { admit. }
-  des.
-
-  exploit (linearize events); eauto. i. des. rename l' into steps.
-
-  (* TODO: https://github.com/kaist-cp/promising-hw/issues/46#issuecomment-672911617 4. *)
-  admit.
 Admitted.
